added abstract/concrete encodings of array_max and array_min

examples/pseudo_bool/cp_encoding/cp_to_ilpScript.sml
@@ -63,6 +63,10 @@ Definition reify_flag_def:
       else if ann = SOME (strlit"eq")
       then varc wi (EL (EL 0 ids) Xs) = EL (EL 1 ids) iS
       else MEM (varc wi (EL (HD ids) Xs)) iS (* ann = SOME (strlit"fnd") *)
+    | SOME (Array (ArrayMax Xs Y)) =>
+      varc wi (EL (HD ids) Xs) ≥ varc wi Y
+    | SOME (Array (ArrayMin Xs Y)) =>
+      varc wi (EL (HD ids) Xs) ≤ varc wi Y
     | SOME (Extensional (Table tss Xs)) =>
       match_row (EL (HD ids) tss) (MAP (varc wi) Xs))
   | Flag ann =>
